# baseURI: http://www.connaissance.io/onto/cd/CourseDesign
# imports: http://data.opendiscoveryspace.eu/lom_ontology_ods.owl#
# imports: http://topbraid.org/schema/

@prefix : <http://www.connaissance.io/onto/cd/CourseDesign#> .
@prefix dcterms: <http://purl.org/dc/terms/> .
@prefix foaf: <http://xmlns.com/foaf/0.1/> .
@prefix lom_ontology_ods: <http://data.opendiscoveryspace.eu/lom_ontology_ods.owl#> .
@prefix owl: <http://www.w3.org/2002/07/owl#> .
@prefix rdf: <http://www.w3.org/1999/02/22-rdf-syntax-ns#> .
@prefix rdfs: <http://www.w3.org/2000/01/rdf-schema#> .
@prefix schema: <http://schema.org/> .
@prefix skos: <http://www.w3.org/2004/02/skos/core#> .
@prefix xsd: <http://www.w3.org/2001/XMLSchema#> .

schema:Course
  rdf:type owl:Class ;
  schema:provider schema:CollegeOrUniversity ;
  rdfs:comment "A description of an educational course which may be offered as distinct instances at which take place at different times or take place at different locations, or be offered through different media or modes of study. An educational course is a sequence of one or more educational events and/or creative works which aims to build knowledge, competence or ability of learners." ;
  rdfs:label "Course" ;
  rdfs:subClassOf schema:CreativeWork ;
  rdfs:subClassOf schema:EducationEvent ;
.
<http://www.connaissance.io/onto/cd/CourseDesign>
  rdf:type owl:Ontology ;
  dcterms:creator :M_Lane ;
  dcterms:modified "2021-09-12" ;
  rdfs:comment "Ontology for structured instructional design; imports IEEE LOM." ;
  owl:imports lom_ontology_ods: ;
  owl:imports <http://topbraid.org/schema/> ;
.
:Course_Assignments
  rdf:type owl:Class ;
  rdfs:comment "Specific due dates for all assignments in the course." ;
  rdfs:label "Assignment & Due Dates" ;
  rdfs:subClassOf schema:Course ;
  rdfs:subClassOf schema:Intangible ;
.
:Course_Description
  rdf:type owl:Class ;
  rdfs:comment "A narrative describing the course; i.e., purpose, goals, general prerequisites." ;
  rdfs:label "Course Description" ;
  rdfs:subClassOf schema:Course ;
  rdfs:subClassOf schema:Intangible ;
.
:Course_Evaluation
  rdf:type owl:Class ;
  rdfs:comment "The official quality assurance evaluation for the course." ;
  rdfs:label "Course Evaluation" ;
  rdfs:subClassOf schema:Course ;
  rdfs:subClassOf schema:Intangible ;
.
:Course_Expectations
  rdf:type owl:Class ;
  rdfs:comment "A narrative asserting instructor expectations and requirements for the course." ;
  rdfs:label "Course Expectations & Requirements" ;
  rdfs:subClassOf schema:Course ;
  rdfs:subClassOf schema:Intangible ;
.
:Course_Format
  rdf:type owl:Class ;
  rdfs:comment "Delivery format specified for the course." ;
  rdfs:label "Course Format" ;
  rdfs:subClassOf schema:Course ;
  rdfs:subClassOf schema:Intangible ;
.
:Course_Grading
  rdf:type owl:Class ;
  rdfs:comment "Grading methods and success criteria specified for the course." ;
  rdfs:label "Course Description" ;
  rdfs:subClassOf schema:Course ;
  rdfs:subClassOf schema:Intangible ;
.
:Course_Objectives
  rdf:type owl:Class ;
  rdfs:comment "The set of measurable learning objectives for the course or learning module." ;
  rdfs:label "Course Learning Objectives" ;
  rdfs:subClassOf schema:Course ;
  rdfs:subClassOf schema:Intangible ;
.
:Course_Prerequisites
  rdf:type owl:Class ;
  rdfs:comment "Specific knowledge, skills, and possible courses required in advance of course." ;
  rdfs:label "Course Prerequisites" ;
  rdfs:subClassOf schema:Course ;
  rdfs:subClassOf schema:Intangible ;
.
:Course_Readings
  rdf:type owl:Class ;
  rdfs:comment "Reading assignments in the course." ;
  rdfs:label "Course Readings & Topics" ;
  rdfs:subClassOf schema:Course ;
  rdfs:subClassOf schema:Intangible ;
.
:Course_Schedule
  rdf:type owl:Class ;
  rdfs:comment "Specific schedule of learning topics, units, activities, assessments, and due dates." ;
  rdfs:label "Course Schedule" ;
  rdfs:subClassOf schema:Course ;
  rdfs:subClassOf schema:Intangible ;
.
:Course_Technology
  rdf:type owl:Class ;
  rdfs:comment "Technology and software requirements for the course." ;
  rdfs:label "Course Technology & Software Requirements" ;
  rdfs:subClassOf schema:Course ;
  rdfs:subClassOf schema:Intangible ;
.
:Instructor_Bio
  rdf:type owl:Class ;
  rdfs:comment "A narrative of the instructor's background as it relates to the course." ;
  rdfs:label "Instructor Bio" ;
  rdfs:subClassOf schema:Course ;
  rdfs:subClassOf schema:Intangible ;
.
:Learning_Module
  rdf:type owl:Class ;
  rdfs:comment "All inclusive learning module for the course." ;
  rdfs:label "Learning Module" ;
  rdfs:subClassOf schema:Course ;
  rdfs:subClassOf schema:Intangible ;
.
:M_Lane
  rdf:type schema:Person ;
  rdfs:label "M Laner" ;
.
:Module_Assessment
  rdf:type owl:Class ;
  rdfs:comment "Graded assessment for the module." ;
  rdfs:label "Module Assessment" ;
  rdfs:subClassOf schema:Intangible ;
  rdfs:subClassOf :Learning_Module ;
.
:Module_Assignment
  rdf:type owl:Class ;
  rdfs:comment "Graded assignment instructions for the module." ;
  rdfs:label "Module Assignment" ;
  rdfs:subClassOf schema:Intangible ;
  rdfs:subClassOf :Learning_Module ;
.
:Module_Description
  rdf:type owl:Class ;
  rdfs:comment "A narrative describing the learning module; i.e., purpose, goals, general prerequisites." ;
  rdfs:label "Module Description" ;
  rdfs:subClassOf schema:Intangible ;
  rdfs:subClassOf :Learning_Module ;
.
:Module_Discussion
  rdf:type owl:Class ;
  rdfs:comment "Discussion questions for the module." ;
  rdfs:label "Module Discussion Questions" ;
  rdfs:subClassOf schema:Intangible ;
  rdfs:subClassOf :Learning_Module ;
.
:Module_Lecture
  rdf:type owl:Class ;
  rdfs:comment "Module lecture materials in multimedia format, including plain old text." ;
  rdfs:label "Module Lecture" ;
  rdfs:subClassOf schema:Intangible ;
  rdfs:subClassOf :Learning_Module ;
.
:Module_Objectives
  rdf:type owl:Class ;
  rdfs:comment "The set of measurable learning objectives for the learning module." ;
  rdfs:label "Module Learning Objectives" ;
  rdfs:subClassOf schema:Intangible ;
  rdfs:subClassOf :Learning_Module ;
.
:Module_Readings
  rdf:type owl:Class ;
  rdfs:comment "Reading and media assignments for the module." ;
  rdfs:label "Module Readings & Media" ;
  rdfs:subClassOf schema:Intangible ;
  rdfs:subClassOf :Learning_Module ;
.
