# baseURI: http://data.opendiscoveryspace.eu/lom_ontology_ods.owl#
# prefix: lom2owl

@prefix : <http://data.opendiscoveryspace.eu/lom_ontology_ods.owl#> .
@prefix cc: <http://creativecommons.org/ns#> .
@prefix dc: <http://purl.org/dc/elements/1.1/> .
@prefix lom2owl: <http://data.opendiscoveryspace.eu/lom_ontology_ods.owl#> .
@prefix ns: <http://www.w3.org/2006/vcard/ns#> .
@prefix owl: <http://www.w3.org/2002/07/owl#> .
@prefix owl2xml: <http://www.w3.org/2006/12/owl2-xml#> .
@prefix rdf: <http://www.w3.org/1999/02/22-rdf-syntax-ns#> .
@prefix rdfs: <http://www.w3.org/2000/01/rdf-schema#> .
@prefix terms: <http://purl.org/dc/terms/> .
@prefix xsd: <http://www.w3.org/2001/XMLSchema#> .

lom2owl:
  rdf:type owl:Ontology ;
  cc:license <http://creativecommons.org/licenses/by/3.0/> ;
  dc:creator "Enayat Rajabi (enayat.rajabi@uah.es)" ;
  dc:description """An ontology and vocabulary used for exposing IEEE LOM, a metadata standard for educational contents, as Linked Data. 
		It is intended as a bridge for linkage of educational metadata into Linked Open Data (LOD). 
		In this ontology, we designed a mapping of IEEE LOM elements to RDF based on Linked Data principles. """@en ;
  dc:issued "2014-05-20"^^xsd:date ;
  dc:modified "2015-03-30"^^xsd:date ;
  dc:publisher "University of Alcala (www.uah.es) " ;
  dc:rights "Copyright Â© 2015 University of Alcala, Information Engineering (IE) research unit (http://www.ieru.org/) " ;
  dc:title "A vocabulary for exposing IEEE LOM metadata as Linked Open Data"@en ;
  rdfs:comment "-Version 1.0: covers a complete mapping of IEEE LOM to Linked Open Data"@en ;
  owl:versionInfo 1.0 ;
.
lom2owl:Annotation
  rdf:type owl:Class ;
  rdfs:comment "Comments on the educational use of a learning object, including information on when and by whom the comments were created."@en ;
  rdfs:subClassOf owl:Thing ;
  rdfs:subClassOf [
      rdf:type owl:Restriction ;
      owl:cardinality "1"^^xsd:nonNegativeInteger ;
      owl:onProperty lom2owl:dateTimeDescription ;
    ] ;
  rdfs:subClassOf [
      rdf:type owl:Restriction ;
      owl:cardinality "1"^^xsd:nonNegativeInteger ;
      owl:onProperty lom2owl:dateTimeValue ;
    ] ;
  rdfs:subClassOf [
      rdf:type owl:Restriction ;
      owl:onClass lom2owl:VCard ;
      owl:onProperty lom2owl:annotationEntity ;
      owl:qualifiedCardinality "1"^^xsd:nonNegativeInteger ;
    ] ;
  rdfs:subClassOf [
      rdf:type owl:Restriction ;
      owl:onProperty lom2owl:annotationDescription ;
      owl:someValuesFrom rdfs:Literal ;
    ] ;
.
lom2owl:Classification
  rdf:type owl:Class ;
  rdfs:comment "Description of where a learning object falls within a particular classification system. To define multiple classifications, there may be multiple instances of this category for a learning object."@en ;
  rdfs:subClassOf owl:Thing ;
  rdfs:subClassOf [
      rdf:type owl:Restriction ;
      owl:cardinality "1"^^xsd:nonNegativeInteger ;
      owl:onProperty lom2owl:classificationPurpose ;
    ] ;
  rdfs:subClassOf [
      rdf:type owl:Restriction ;
      owl:maxQualifiedCardinality "15"^^xsd:nonNegativeInteger ;
      owl:onClass lom2owl:TaxonPath ;
      owl:onProperty lom2owl:taxonPath ;
    ] ;
  rdfs:subClassOf [
      rdf:type owl:Restriction ;
      owl:maxQualifiedCardinality "40"^^xsd:nonNegativeInteger ;
      owl:onClass lom2owl:LangString ;
      owl:onProperty lom2owl:classificationKeyword ;
    ] ;
  rdfs:subClassOf [
      rdf:type owl:Restriction ;
      owl:onProperty lom2owl:classificationDescription ;
      owl:someValuesFrom rdfs:Literal ;
    ] ;
.
lom2owl:Contribution
  rdf:type owl:Class ;
  rdfs:comment "Those entities (i.e., people, organizations) that have contributed to the state of this learning object during its life cycle (e.g., creation, edits, publication)." ;
  rdfs:subClassOf owl:Thing ;
.
lom2owl:DateTime
  rdf:type owl:Class ;
  rdfs:comment "A point in time with accuracy at least as small as one second, as described by IEEE LOM in clause 8 (IEEE 1484.12.1-2002)."@en ;
  rdfs:subClassOf owl:Thing ;
  rdfs:subClassOf [
      rdf:type owl:Restriction ;
      owl:onDataRange xsd:dateTime ;
      owl:onProperty lom2owl:dateTimeValue ;
      owl:qualifiedCardinality "1"^^xsd:nonNegativeInteger ;
    ] ;
.
lom2owl:Duration
  rdf:type owl:Class ;
  rdfs:comment "An interval in time with accuracy at least as small as one second."@en ;
  rdfs:subClassOf owl:Thing ;
  rdfs:subClassOf [
      rdf:type owl:Restriction ;
      owl:onDataRange rdf:XMLLiteral ;
      owl:onProperty lom2owl:durationDescription ;
      owl:qualifiedCardinality "1"^^xsd:nonNegativeInteger ;
    ] ;
  rdfs:subClassOf [
      rdf:type owl:Restriction ;
      owl:onDataRange rdf:XMLLiteral ;
      owl:onProperty lom2owl:durationValue ;
      owl:qualifiedCardinality "1"^^xsd:nonNegativeInteger ;
    ] ;
.
lom2owl:Educational
  rdf:type owl:Class ;
  terms:type ""^^rdfs:Literal ;
  rdfs:subClassOf owl:Thing ;
  rdfs:subClassOf [
      rdf:type owl:Restriction ;
      owl:cardinality "1"^^xsd:nonNegativeInteger ;
      owl:onProperty lom2owl:educationalDifficulty ;
    ] ;
  rdfs:subClassOf [
      rdf:type owl:Restriction ;
      owl:cardinality "1"^^xsd:nonNegativeInteger ;
      owl:onProperty lom2owl:educationalInteractivityLevel ;
    ] ;
  rdfs:subClassOf [
      rdf:type owl:Restriction ;
      owl:cardinality "1"^^xsd:nonNegativeInteger ;
      owl:onProperty lom2owl:educationalInteractivityType ;
    ] ;
  rdfs:subClassOf [
      rdf:type owl:Restriction ;
      owl:cardinality "1"^^xsd:nonNegativeInteger ;
      owl:onProperty lom2owl:educationalSemanticDensity ;
    ] ;
  rdfs:subClassOf [
      rdf:type owl:Restriction ;
      owl:maxCardinality "10"^^xsd:nonNegativeInteger ;
      owl:onProperty lom2owl:educationalContext ;
    ] ;
  rdfs:subClassOf [
      rdf:type owl:Restriction ;
      owl:maxCardinality "10"^^xsd:nonNegativeInteger ;
      owl:onProperty lom2owl:educationalIntendedUserRole ;
    ] ;
  rdfs:subClassOf [
      rdf:type owl:Restriction ;
      owl:maxCardinality "10"^^xsd:nonNegativeInteger ;
      owl:onProperty lom2owl:educationalLanguage ;
    ] ;
  rdfs:subClassOf [
      rdf:type owl:Restriction ;
      owl:maxQualifiedCardinality "10"^^xsd:nonNegativeInteger ;
      owl:onClass lom2owl:LangString ;
      owl:onProperty lom2owl:description ;
    ] ;
  rdfs:subClassOf [
      rdf:type owl:Restriction ;
      owl:maxQualifiedCardinality "5"^^xsd:nonNegativeInteger ;
      owl:onClass lom2owl:LangString ;
      owl:onProperty lom2owl:educationalTypicalAgeRange ;
    ] ;
  rdfs:subClassOf [
      rdf:type owl:Restriction ;
      owl:onClass lom2owl:Duration ;
      owl:onProperty lom2owl:educationalTypicalLearningTime ;
      owl:qualifiedCardinality "1"^^xsd:nonNegativeInteger ;
    ] ;
.
lom2owl:Identifier
  rdf:type owl:Class ;
  terms:identifier ""^^rdfs:Literal ;
  rdfs:comment "A globally unique label that identifies either a learning object or a learning object metadata record."@en ;
  rdfs:subClassOf owl:Thing ;
  rdfs:subClassOf [
      rdf:type owl:Restriction ;
      owl:cardinality "1"^^xsd:nonNegativeInteger ;
      owl:onProperty lom2owl:identifierCatalog ;
    ] ;
.
lom2owl:LangString
  rdf:type owl:Class ;
  rdfs:comment "Each of the possible semantically equivalent character strings of a langString."@en ;
  rdfs:subClassOf owl:Thing ;
  rdfs:subClassOf [
      rdf:type owl:Restriction ;
      owl:onProperty lom2owl:hasValue ;
      owl:someValuesFrom rdfs:Literal ;
    ] ;
.
lom2owl:LearningObject
  rdf:type owl:Class ;
  terms:format ""^^rdfs:Literal ;
  terms:language ""^^rdfs:Literal ;
  terms:publisher ""^^rdfs:Literal ;
  terms:rights ""^^rdfs:Literal ;
  rdfs:comment "Learning Object" ;
  rdfs:subClassOf owl:Thing ;
  rdfs:subClassOf [
      rdf:type owl:Restriction ;
      owl:cardinality "1"^^xsd:nonNegativeInteger ;
      owl:onProperty lom2owl:aggregationLevel ;
    ] ;
  rdfs:subClassOf [
      rdf:type owl:Restriction ;
      owl:cardinality "1"^^xsd:nonNegativeInteger ;
      owl:onProperty lom2owl:lifeCycleStatus ;
    ] ;
  rdfs:subClassOf [
      rdf:type owl:Restriction ;
      owl:cardinality "1"^^xsd:nonNegativeInteger ;
      owl:onProperty lom2owl:metaMetadataLanguage ;
    ] ;
  rdfs:subClassOf [
      rdf:type owl:Restriction ;
      owl:cardinality "1"^^xsd:nonNegativeInteger ;
      owl:onProperty lom2owl:structure ;
    ] ;
  rdfs:subClassOf [
      rdf:type owl:Restriction ;
      owl:cardinality "1"^^xsd:nonNegativeInteger ;
      owl:onProperty lom2owl:technicalSize ;
    ] ;
  rdfs:subClassOf [
      rdf:type owl:Restriction ;
      owl:maxCardinality "10"^^xsd:nonNegativeInteger ;
      owl:onProperty lom2owl:metadataSchema ;
    ] ;
  rdfs:subClassOf [
      rdf:type owl:Restriction ;
      owl:maxCardinality "10"^^xsd:nonNegativeInteger ;
      owl:onProperty lom2owl:technicalLocation ;
    ] ;
  rdfs:subClassOf [
      rdf:type owl:Restriction ;
      owl:maxQualifiedCardinality "10"^^xsd:nonNegativeInteger ;
      owl:onClass lom2owl:Identifier ;
      owl:onProperty lom2owl:identifier ;
    ] ;
  rdfs:subClassOf [
      rdf:type owl:Restriction ;
      owl:maxQualifiedCardinality "10"^^xsd:nonNegativeInteger ;
      owl:onClass lom2owl:Identifier ;
      owl:onProperty lom2owl:metaMetadataIdentifier ;
    ] ;
  rdfs:subClassOf [
      rdf:type owl:Restriction ;
      owl:maxQualifiedCardinality "10"^^xsd:nonNegativeInteger ;
      owl:onClass lom2owl:LangString ;
      owl:onProperty lom2owl:coverage ;
    ] ;
  rdfs:subClassOf [
      rdf:type owl:Restriction ;
      owl:maxQualifiedCardinality "10"^^xsd:nonNegativeInteger ;
      owl:onClass lom2owl:LangString ;
      owl:onProperty lom2owl:description ;
    ] ;
  rdfs:subClassOf [
      rdf:type owl:Restriction ;
      owl:maxQualifiedCardinality "10"^^xsd:nonNegativeInteger ;
      owl:onClass lom2owl:LangString ;
      owl:onProperty lom2owl:keyword ;
    ] ;
  rdfs:subClassOf [
      rdf:type owl:Restriction ;
      owl:maxQualifiedCardinality "10"^^xsd:nonNegativeInteger ;
      owl:onClass lom2owl:MetaMetadataContribution ;
      owl:onProperty lom2owl:metaMetadataContribution ;
    ] ;
  rdfs:subClassOf [
      rdf:type owl:Restriction ;
      owl:maxQualifiedCardinality "100"^^xsd:nonNegativeInteger ;
      owl:onClass lom2owl:Educational ;
      owl:onProperty lom2owl:educational ;
    ] ;
  rdfs:subClassOf [
      rdf:type owl:Restriction ;
      owl:maxQualifiedCardinality "100"^^xsd:nonNegativeInteger ;
      owl:onClass lom2owl:Relation ;
      owl:onProperty lom2owl:relation ;
    ] ;
  rdfs:subClassOf [
      rdf:type owl:Restriction ;
      owl:maxQualifiedCardinality "30"^^xsd:nonNegativeInteger ;
      owl:onClass lom2owl:Annotation ;
      owl:onProperty lom2owl:annotation ;
    ] ;
  rdfs:subClassOf [
      rdf:type owl:Restriction ;
      owl:maxQualifiedCardinality "30"^^xsd:nonNegativeInteger ;
      owl:onClass lom2owl:LifeCycleContribution ;
      owl:onProperty lom2owl:lifeCycleContribution ;
    ] ;
  rdfs:subClassOf [
      rdf:type owl:Restriction ;
      owl:maxQualifiedCardinality "40"^^xsd:nonNegativeInteger ;
      owl:onClass lom2owl:Classification ;
      owl:onProperty lom2owl:classification ;
    ] ;
  rdfs:subClassOf [
      rdf:type owl:Restriction ;
      owl:maxQualifiedCardinality "40"^^xsd:nonNegativeInteger ;
      owl:onClass lom2owl:TechnicalRequirement ;
      owl:onProperty lom2owl:technicalRequirements ;
    ] ;
  rdfs:subClassOf [
      rdf:type owl:Restriction ;
      owl:onClass lom2owl:Duration ;
      owl:onProperty lom2owl:technicalDuration ;
      owl:qualifiedCardinality "1"^^xsd:nonNegativeInteger ;
    ] ;
  rdfs:subClassOf [
      rdf:type owl:Restriction ;
      owl:onDataRange xsd:boolean ;
      owl:onProperty lom2owl:copyrightAndOtherRestrictions ;
      owl:qualifiedCardinality "1"^^xsd:nonNegativeInteger ;
    ] ;
  rdfs:subClassOf [
      rdf:type owl:Restriction ;
      owl:onDataRange xsd:boolean ;
      owl:onProperty lom2owl:cost ;
      owl:qualifiedCardinality "1"^^xsd:nonNegativeInteger ;
    ] ;
  rdfs:subClassOf [
      rdf:type owl:Restriction ;
      owl:onProperty lom2owl:lifeCycleVersion ;
      owl:someValuesFrom rdfs:Literal ;
    ] ;
  rdfs:subClassOf [
      rdf:type owl:Restriction ;
      owl:onProperty lom2owl:otherPlatformRequirements ;
      owl:someValuesFrom rdfs:Literal ;
    ] ;
  rdfs:subClassOf [
      rdf:type owl:Restriction ;
      owl:onProperty lom2owl:technicalInstallationRemarks ;
      owl:someValuesFrom rdfs:Literal ;
    ] ;
.
lom2owl:LifeCycleContribution
  rdf:type owl:Class ;
  rdfs:subClassOf lom2owl:Contribution ;
  rdfs:subClassOf [
      rdf:type owl:Restriction ;
      owl:cardinality "1"^^xsd:nonNegativeInteger ;
      owl:onProperty lom2owl:dateTimeDescription ;
    ] ;
  rdfs:subClassOf [
      rdf:type owl:Restriction ;
      owl:cardinality "1"^^xsd:nonNegativeInteger ;
      owl:onProperty lom2owl:dateTimeValue ;
    ] ;
  rdfs:subClassOf [
      rdf:type owl:Restriction ;
      owl:maxCardinality "1"^^xsd:nonNegativeInteger ;
      owl:onProperty lom2owl:lifeCycleContributionRole ;
    ] ;
.
lom2owl:MetaMetadataContribution
  rdf:type owl:Class ;
  rdfs:subClassOf lom2owl:Contribution ;
  rdfs:subClassOf [
      rdf:type owl:Restriction ;
      owl:cardinality "1"^^xsd:nonNegativeInteger ;
      owl:onProperty lom2owl:dateTimeDescription ;
    ] ;
  rdfs:subClassOf [
      rdf:type owl:Restriction ;
      owl:cardinality "1"^^xsd:nonNegativeInteger ;
      owl:onProperty lom2owl:dateTimeValue ;
    ] ;
  rdfs:subClassOf [
      rdf:type owl:Restriction ;
      owl:maxCardinality "1"^^xsd:nonNegativeInteger ;
      owl:onProperty lom2owl:metaMetadataContributionRole ;
    ] ;
.
lom2owl:Relation
  rdf:type owl:Class ;
  rdfs:comment "A concept which defines the relationship between a learning object and other learning objects, if any."@en ;
  rdfs:subClassOf owl:Thing ;
  rdfs:subClassOf [
      rdf:type owl:Restriction ;
      owl:cardinality "1"^^xsd:nonNegativeInteger ;
      owl:onProperty lom2owl:relationKind ;
    ] ;
  rdfs:subClassOf [
      rdf:type owl:Restriction ;
      owl:maxQualifiedCardinality "10"^^xsd:nonNegativeInteger ;
      owl:onClass lom2owl:Identifier ;
      owl:onProperty lom2owl:identifier ;
    ] ;
  rdfs:subClassOf [
      rdf:type owl:Restriction ;
      owl:maxQualifiedCardinality "10"^^xsd:nonNegativeInteger ;
      owl:onClass lom2owl:LangString ;
      owl:onProperty lom2owl:relatedResourceDescription ;
    ] ;
.
lom2owl:SingleTechnicalRequirement
  rdf:type owl:Class ;
  rdfs:comment "A technical capability necessary for using a learning object."@en ;
  rdfs:subClassOf owl:Thing ;
  rdfs:subClassOf [
      rdf:type owl:Restriction ;
      owl:cardinality "1"^^xsd:nonNegativeInteger ;
      owl:onProperty lom2owl:orCompositeName ;
    ] ;
  rdfs:subClassOf [
      rdf:type owl:Restriction ;
      owl:cardinality "1"^^xsd:nonNegativeInteger ;
      owl:onProperty lom2owl:orCompositeType ;
    ] ;
  rdfs:subClassOf [
      rdf:type owl:Restriction ;
      owl:maxCardinality "1"^^xsd:nonNegativeInteger ;
      owl:onProperty lom2owl:orCompositeMaximumVersion ;
    ] ;
  rdfs:subClassOf [
      rdf:type owl:Restriction ;
      owl:maxCardinality "1"^^xsd:nonNegativeInteger ;
      owl:onProperty lom2owl:orCompositeMinimumVersion ;
    ] ;
.
lom2owl:Taxon
  rdf:type owl:Class ;
  rdfs:comment """A particular term within a taxonomy. A taxon is a node that has a defined label or
term. A taxon may also have an alphanumeric designation or identifier for standardized reference. Either or both the label and the entry may be used to designate a particular taxon. An ordered list of taxons creates a taxonomic path, i.e., \"taxonomic stairway\": this is a path from a more general to more specific entry in a classification."""@en ;
  rdfs:subClassOf owl:Thing ;
  rdfs:subClassOf [
      rdf:type owl:Restriction ;
      owl:cardinality "1"^^xsd:nonNegativeInteger ;
      owl:onProperty lom2owl:taxonId ;
    ] ;
  rdfs:subClassOf [
      rdf:type owl:Restriction ;
      owl:onProperty lom2owl:taxonEntry ;
      owl:someValuesFrom rdfs:Literal ;
    ] ;
.
lom2owl:TaxonPath
  rdf:type owl:Class ;
  rdfs:comment "A taxonomic path in a specific classification system. Each succeeding level is a refinement in the definition of the preceding level. There may be different paths, in the same or different classifications, which describe the same characteristic."@en ;
  rdfs:subClassOf owl:Thing ;
  rdfs:subClassOf [
      rdf:type owl:Restriction ;
      owl:maxQualifiedCardinality "15"^^xsd:nonNegativeInteger ;
      owl:onClass lom2owl:Taxon ;
      owl:onProperty lom2owl:classificationTaxon ;
    ] ;
  rdfs:subClassOf [
      rdf:type owl:Restriction ;
      owl:onProperty lom2owl:taxonpathSource ;
      owl:someValuesFrom rdfs:Literal ;
    ] ;
.
lom2owl:TechnicalRequirement
  rdf:type owl:Class ;
  rdfs:comment "The technical capabilities necessary for using a learning object. There can be multiple requirements, in which case all are required, i.e., the logical connector is AND."@en ;
  rdfs:subClassOf owl:Thing ;
  rdfs:subClassOf [
      rdf:type owl:Restriction ;
      owl:maxQualifiedCardinality "40"^^xsd:nonNegativeInteger ;
      owl:onClass lom2owl:SingleTechnicalRequirement ;
      owl:onProperty lom2owl:isCompositeOf ;
    ] ;
.
lom2owl:VCard
  rdf:type owl:Class ;
  rdfs:comment "A vCard is a collection of one or more properties. A property is a uniquely named value. A set of properties can be grouped within a vCard. For example, the properties for a telephone number and comment can be grouped in order to preserve the coupling of the annotation with the telephone number. In addition to property groupings, a vC. versit  is developing a comprehensive family of PDI technologies based on open specifications and interoperability agreements to help meet this technology need." ;
  rdfs:subClassOf owl:Thing ;
  ns:FN ""^^rdfs:Literal ;
  ns:N ""^^rdfs:Literal ;
  ns:ORG ""^^rdfs:Literal ;
  ns:email ""^^rdfs:Literal ;
.
lom2owl:aggregationLevel
  rdf:type owl:DatatypeProperty ;
  rdfs:comment "The functional granularity of this learning object. IEEE LOM element 1.8."@en ;
  rdfs:domain lom2owl:LearningObject ;
  rdfs:range [
      rdf:type owl:DataRange ;
      owl:oneOf [
          rdf:type rdf:List ;
          rdf:first "1" ;
          rdf:rest [
              rdf:type rdf:List ;
              rdf:first "2" ;
              rdf:rest [
                  rdf:type rdf:List ;
                  rdf:first "3" ;
                  rdf:rest [
                      rdf:type rdf:List ;
                      rdf:first "4" ;
                      rdf:rest () ;
                    ] ;
                ] ;
            ] ;
        ] ;
    ] ;
.
lom2owl:annotation
  rdf:type owl:ObjectProperty ;
  rdfs:comment "Comments on the educational use of a learning object, containing information on when and by whom the comments were created. This category enables educators to share their assessments of learning objects, suggestions for use, etc. IEEE LOM element 8."@en ;
  rdfs:range lom2owl:Annotation ;
.
lom2owl:annotationDate
  rdf:type owl:ObjectProperty ;
  rdfs:comment "Date that this annotation was created. IEEE LOM element 8.2."@en ;
  rdfs:domain lom2owl:Annotation ;
  rdfs:range lom2owl:DateTime ;
.
lom2owl:annotationDescription
  rdf:type owl:DatatypeProperty ;
  rdfs:domain lom2owl:Annotation ;
  rdfs:range rdfs:Literal ;
.
lom2owl:annotationEntity
  rdf:type owl:DatatypeProperty ;
  rdf:type owl:ObjectProperty ;
  rdf:type owl:Thing ;
  rdfs:comment "Entity (i.e., people, organization) that created this annotation. IEEE LOM element 8.1."@en ;
  owl:dataPropertyDomain lom2owl:Annotation ;
  owl:dataPropertyRange xsd:string ;
.
lom2owl:classification
  rdf:type owl:ObjectProperty ;
  rdfs:comment "Description of where a learning object falls within a particular classification system. IEEE LOM element 9."@en ;
  rdfs:range lom2owl:Classification ;
.
lom2owl:classificationDescription
  rdf:type owl:DatatypeProperty ;
  rdfs:domain lom2owl:Classification ;
  rdfs:range rdfs:Literal ;
.
lom2owl:classificationKeyword
  rdf:type owl:ObjectProperty ;
  rdfs:comment "Keywords and phrases descriptive of the learning object relative to the stated 9.1:Classification.Purpose of this specific classification, such as accessibility, security level, etc., most relevant first. IEEE LOM element 9.4" ;
  rdfs:domain lom2owl:Classification ;
.
lom2owl:classificationPurpose
  rdf:type owl:DatatypeProperty ;
  rdfs:comment "The purpose of classifying a learning object. IEEE LOM element 9.1."@en ;
  rdfs:domain lom2owl:Classification ;
  rdfs:range [
      rdf:type owl:DataRange ;
      owl:oneOf [
          rdf:type rdf:List ;
          rdf:first "accessibility" ;
          rdf:rest [
              rdf:type rdf:List ;
              rdf:first "competency" ;
              rdf:rest [
                  rdf:type rdf:List ;
                  rdf:first "discipline" ;
                  rdf:rest [
                      rdf:type rdf:List ;
                      rdf:first "educational level" ;
                      rdf:rest [
                          rdf:type rdf:List ;
                          rdf:first "educational objective" ;
                          rdf:rest [
                              rdf:type rdf:List ;
                              rdf:first "idea" ;
                              rdf:rest [
                                  rdf:type rdf:List ;
                                  rdf:first "prerequisite" ;
                                  rdf:rest [
                                      rdf:type rdf:List ;
                                      rdf:first "restrictions" ;
                                      rdf:rest [
                                          rdf:type rdf:List ;
                                          rdf:first "security level" ;
                                          rdf:rest [
                                              rdf:type rdf:List ;
                                              rdf:first "skill level" ;
                                              rdf:rest () ;
                                            ] ;
                                        ] ;
                                    ] ;
                                ] ;
                            ] ;
                        ] ;
                    ] ;
                ] ;
            ] ;
        ] ;
    ] ;
.
lom2owl:classificationTaxon
  rdf:type owl:ObjectProperty ;
  rdfs:comment "A particular term within a taxonomy which serves to classify a learning object. IEEE LOM element 9.2.2."@en ;
  rdfs:domain lom2owl:TaxonPath ;
  rdfs:range lom2owl:Taxon ;
.
lom2owl:contributionDateTime
  rdf:type owl:ObjectProperty ;
  rdfs:comment "The date of the contribution. IEEE LOM element 3.2.3."@en ;
  rdfs:domain lom2owl:Contribution ;
  rdfs:range lom2owl:DateTime ;
.
lom2owl:contributionEntity
  rdf:type owl:ObjectProperty ;
  rdfs:comment "The identification of and information about entities (i.e., people, organizations) contributing to this learning object. The entities shall be ordered as most relevant first. IEEE LOM element 3.2.2." ;
  rdfs:domain lom2owl:Contribution ;
  rdfs:range lom2owl:VCard ;
.
lom2owl:copyrightAndOtherRestrictions
  rdf:type owl:DatatypeProperty ;
  rdfs:comment "Whether copyright or other restrictions apply to the use of this learning object. IEEE LOM element 6.2."@en ;
  rdfs:range xsd:boolean ;
.
lom2owl:copyrightDescription
  rdf:type owl:DatatypeProperty ;
  rdfs:domain lom2owl:LearningObject ;
  rdfs:range rdfs:Literal ;
.
lom2owl:cost
  rdf:type owl:DatatypeProperty ;
  rdfs:comment "Whether use of the learning object requires payment. IEEE LOM element 6.1."@en ;
  rdfs:range xsd:boolean ;
.
lom2owl:coverage
  rdf:type owl:ObjectProperty ;
  terms:coverage ""^^rdfs:Literal ;
  rdfs:comment """The time, culture, geography or region to which this learning object applies.
The extent or scope of the content of the learning object. Coverage will typically include spatial location (a place name or geographic coordinates), temporal period (a period label, date, or date range) or jurisdiction (such as a named administrative entity). Recommended best practice is to select a value from a controlled vocabulary (for example, the Thesaurus of Geographic Names [TGN]) and that, where appropriate, named places or time periods be used in preference to numeric identifiers such as sets of coordinates or date ranges. IEEE LOM element 1.6."""@en ;
  rdfs:domain lom2owl:LearningObject ;
.
lom2owl:dateTimeDescription
  rdf:type owl:DatatypeProperty ;
  rdfs:domain lom2owl:Contribution ;
  rdfs:range rdfs:Literal ;
.
lom2owl:dateTimeValue
  rdf:type owl:DatatypeProperty ;
  rdfs:comment "Date time value in format: YYYY[-MM[-DD[Thh[:mm[:ss[.s[TZD]]]]]]]"@en ;
  rdfs:domain lom2owl:DateTime ;
  rdfs:range xsd:dateTime ;
.
lom2owl:description
  rdf:type owl:ObjectProperty ;
  terms:description ""^^rdfs:Literal ;
  rdfs:comment "A textual description of the content of this learning object. IEEE LOM element 1.4."@en ;
  rdfs:comment "Comments on how this learning object is to be used. IEEE LOM element 5.10" ;
  rdfs:domain lom2owl:LearningObject ;
.
lom2owl:duration
  rdf:type owl:ObjectProperty ;
  rdfs:domain lom2owl:Duration ;
.
lom2owl:durationDescription
  rdf:type owl:DatatypeProperty ;
  rdfs:domain lom2owl:Duration ;
  rdfs:range rdfs:Literal ;
.
lom2owl:durationValue
  rdf:type owl:DatatypeProperty ;
  rdfs:domain lom2owl:Duration ;
  rdfs:range rdfs:Literal ;
.
lom2owl:educational
  rdf:type owl:ObjectProperty ;
  rdfs:comment "This category describes the key educational or pedagogic characteristics of this learning object. IEEE LOM element 5." ;
  rdfs:domain lom2owl:LearningObject ;
  rdfs:range lom2owl:Educational ;
.
lom2owl:educationalContext
  rdf:type owl:DatatypeProperty ;
  rdfs:comment "The principal environment within which the learning and use of this learning object is intended to take place. IEEE LOM element 5.6."@en ;
  rdfs:domain lom2owl:Educational ;
  rdfs:range rdfs:Literal ;
  rdfs:range xsd:short ;
  rdfs:range [
      rdf:type owl:DataRange ;
      owl:oneOf [
          rdf:type rdf:List ;
          rdf:first "higher education" ;
          rdf:rest [
              rdf:type rdf:List ;
              rdf:first "other" ;
              rdf:rest [
                  rdf:type rdf:List ;
                  rdf:first "school" ;
                  rdf:rest [
                      rdf:type rdf:List ;
                      rdf:first "training" ;
                      rdf:rest () ;
                    ] ;
                ] ;
            ] ;
        ] ;
    ] ;
.
lom2owl:educationalDifficulty
  rdf:type owl:DatatypeProperty ;
  rdfs:comment "How hard it is to work with or through this learning object for the typical intended target audience. IEEE LOM element 5.8"@en ;
  rdfs:domain lom2owl:Educational ;
  rdfs:range [
      rdf:type owl:DataRange ;
      owl:oneOf [
          rdf:type rdf:List ;
          rdf:first "difficult" ;
          rdf:rest [
              rdf:type rdf:List ;
              rdf:first "easy" ;
              rdf:rest [
                  rdf:type rdf:List ;
                  rdf:first "medium" ;
                  rdf:rest [
                      rdf:type rdf:List ;
                      rdf:first "very difficult" ;
                      rdf:rest [
                          rdf:type rdf:List ;
                          rdf:first "very easy" ;
                          rdf:rest () ;
                        ] ;
                    ] ;
                ] ;
            ] ;
        ] ;
    ] ;
.
lom2owl:educationalIntendedUserRole
  rdf:type owl:DatatypeProperty ;
  rdfs:comment "Principal user(s) for which this learning object was designed, most dominant first. IEEE LOM element 5.5."@en ;
  rdfs:domain lom2owl:Educational ;
  rdfs:range [
      rdf:type owl:DataRange ;
      owl:oneOf [
          rdf:type rdf:List ;
          rdf:first "author" ;
          rdf:rest [
              rdf:type rdf:List ;
              rdf:first "learner" ;
              rdf:rest [
                  rdf:type rdf:List ;
                  rdf:first "manager" ;
                  rdf:rest [
                      rdf:type rdf:List ;
                      rdf:first "teacher" ;
                      rdf:rest () ;
                    ] ;
                ] ;
            ] ;
        ] ;
    ] ;
.
lom2owl:educationalInteractivityLevel
  rdf:type owl:DatatypeProperty ;
  rdfs:comment "The degree of interactivity characterizing this learning object. Interactivity in this context refers to the degree to which the learner can influence the aspect or behavior of the learning object. IEEE LOM element 5.3." ;
  rdfs:domain lom2owl:Educational ;
  rdfs:range [
      rdf:type owl:DataRange ;
      owl:oneOf [
          rdf:type rdf:List ;
          rdf:first "high" ;
          rdf:rest [
              rdf:type rdf:List ;
              rdf:first "low" ;
              rdf:rest [
                  rdf:type rdf:List ;
                  rdf:first "medium" ;
                  rdf:rest [
                      rdf:type rdf:List ;
                      rdf:first "very high" ;
                      rdf:rest [
                          rdf:type rdf:List ;
                          rdf:first "very low" ;
                          rdf:rest () ;
                        ] ;
                    ] ;
                ] ;
            ] ;
        ] ;
    ] ;
.
lom2owl:educationalInteractivityType
  rdf:type owl:DatatypeProperty ;
  rdfs:comment "Predominant mode of learning supported by this learning object. IEEE LOM element 5.1."@en ;
  rdfs:domain lom2owl:Educational ;
  rdfs:range [
      rdf:type owl:DataRange ;
      owl:oneOf [
          rdf:type rdf:List ;
          rdf:first "active" ;
          rdf:rest [
              rdf:type rdf:List ;
              rdf:first "expositive" ;
              rdf:rest [
                  rdf:type rdf:List ;
                  rdf:first "mised" ;
                  rdf:rest () ;
                ] ;
            ] ;
        ] ;
    ] ;
.
lom2owl:educationalLanguage
  rdf:type owl:DatatypeProperty ;
  rdfs:comment "The primary human language or languages used within this learning object to communicate to the intended user. If the learning object had no lingual content (as in the case of a picture of the Mona Lisa, for example), then the appropriate value for this data element would be \"none\". IEEE LOM element 1.3."@en ;
  rdfs:domain lom2owl:LearningObject ;
  rdfs:range [
      rdf:type owl:DataRange ;
      owl:oneOf [
          rdf:type rdf:List ;
          rdf:first "ba" ;
          rdf:rest [
              rdf:type rdf:List ;
              rdf:first "ca" ;
              rdf:rest [
                  rdf:type rdf:List ;
                  rdf:first "es" ;
                  rdf:rest [
                      rdf:type rdf:List ;
                      rdf:first "ga" ;
                      rdf:rest [
                          rdf:type rdf:List ;
                          rdf:first "none" ;
                          rdf:rest () ;
                        ] ;
                    ] ;
                ] ;
            ] ;
        ] ;
    ] ;
.
lom2owl:educationalSemanticDensity
  rdf:type owl:DatatypeProperty ;
  rdfs:comment "The degree of conciseness of a learning object. The semantic density of a learning object may be estimated in terms of its size, span, or --in the case of self-timed resources such as audio or video-- duration. IEEE LOM element 5.4." ;
  rdfs:domain lom2owl:Educational ;
  rdfs:range xsd:string ;
  rdfs:range [
      rdf:type owl:DataRange ;
      owl:oneOf [
          rdf:type rdf:List ;
          rdf:first "high" ;
          rdf:rest [
              rdf:type rdf:List ;
              rdf:first "low" ;
              rdf:rest [
                  rdf:type rdf:List ;
                  rdf:first "medium" ;
                  rdf:rest [
                      rdf:type rdf:List ;
                      rdf:first "very high" ;
                      rdf:rest [
                          rdf:type rdf:List ;
                          rdf:first "very low" ;
                          rdf:rest () ;
                        ] ;
                    ] ;
                ] ;
            ] ;
        ] ;
    ] ;
  rdfs:range [
      rdf:type owl:DataRange ;
      owl:oneOf [
          rdf:type rdf:List ;
          rdf:first "higherEducation" ;
          rdf:rest [
              rdf:type rdf:List ;
              rdf:first "other" ;
              rdf:rest [
                  rdf:type rdf:List ;
                  rdf:first "school" ;
                  rdf:rest [
                      rdf:type rdf:List ;
                      rdf:first "training" ;
                      rdf:rest () ;
                    ] ;
                ] ;
            ] ;
        ] ;
    ] ;
.
lom2owl:educationalTypicalAgeRange
  rdf:type owl:ObjectProperty ;
  rdf:value ""^^rdfs:Literal ;
  rdfs:comment "Age of the typical intended user. IEEE LOM element 5.7." ;
  rdfs:domain lom2owl:Educational ;
.
lom2owl:educationalTypicalLearningTime
  rdf:type owl:ObjectProperty ;
  rdfs:domain lom2owl:Educational ;
  rdfs:range lom2owl:Duration ;
.
lom2owl:email
  rdf:type owl:DatatypeProperty ;
  rdfs:comment "Email as it appears in the vCard" ;
  rdfs:domain lom2owl:VCard ;
  rdfs:range xsd:string ;
.
lom2owl:hasRelatedResource
  rdf:type owl:ObjectProperty ;
  rdfs:comment "The target learning object that a relationship references. IEEE LOM element 7.2."@en ;
  rdfs:domain lom2owl:Relation ;
  rdfs:range lom2owl:Identifier ;
.
lom2owl:hasResourceIdentifier
  rdf:type owl:ObjectProperty ;
  rdfs:comment "A globally unique label that identifies the target  learning object. IEEE LOM element 7.2.1."@en ;
  rdfs:range lom2owl:Identifier ;
.
lom2owl:hasTechnicalFormat
  rdf:type owl:DatatypeProperty ;
  rdfs:comment "Technical datatype(s) of (all the components of) this learning object. This information is used to identify the software needed to access the learning object. IEEE LOM element 4.1."@en ;
  rdfs:domain lom2owl:LearningObject ;
  rdfs:range xsd:string ;
.
lom2owl:hasValue
  rdf:type owl:DatatypeProperty ;
  rdfs:comment "This predicate relates a singleLangString to the character string containing its textual description."@en ;
  rdfs:range xsd:string ;
.
lom2owl:identifier
  rdf:type owl:InverseFunctionalProperty ;
  rdf:type owl:ObjectProperty ;
  rdfs:comment "This predicate represents the fact that a learning object has a label that identifies it. IEEE LOM element 1.1."@en ;
  rdfs:domain lom2owl:LearningObject ;
  rdfs:range lom2owl:Identifier ;
.
lom2owl:identifierCatalog
  rdf:type owl:DatatypeProperty ;
  rdf:type owl:FunctionalProperty ;
  rdfs:comment "This predicate relates a lomIdentifier to the name or designator of the identification or cataloging scheme used for its identification. It is usually a namespace scheme. IEEE LOM element 1.1, 3.1, 7.2.1."@en ;
  rdfs:domain lom2owl:Identifier ;
  rdfs:range xsd:string ;
.
lom2owl:identifierEntry
  rdf:type owl:DatatypeProperty ;
  rdf:type owl:FunctionalProperty ;
  rdfs:comment "This predicate relates a lomIdentifier to the value of the identifier within the identification or cataloging scheme that designates or identifies a learning object or a learning object metadata record (a namespace specific string).  IEEE LOM element 1.1, 3.1, 7.2.1."@en ;
  rdfs:domain lom2owl:Identifier ;
  rdfs:range xsd:string ;
.
lom2owl:includesSingleLangString
  rdf:type owl:ObjectProperty ;
  rdfs:comment "LangString values may include multiple semantically equivalent character strings, such as translations or alternative descriptions. Each of these is represented by a singleLangString."@en ;
  rdfs:range lom2owl:LangString ;
.
lom2owl:isCompositeOf
  rdf:type owl:ObjectProperty ;
  rdfs:comment "When grouping multiple requirements, the composite requirement is satisfied when one of the component requirements is satisfied, i.e., the logical connector is OR. IEEE LOM element 4.4.1."@en ;
  rdfs:domain lom2owl:TechnicalRequirement ;
  rdfs:range lom2owl:SingleTechnicalRequirement ;
.
lom2owl:keyword
  rdf:type owl:ObjectProperty ;
  rdf:value ""^^rdfs:Literal ;
  rdfs:comment "A keyword or phrase describing the topic of this learning object. This data element should not be used for characteristics that can be described by other data elements. IEEE LOM element 1.5."@en ;
  rdfs:domain lom2owl:LearningObject ;
.
lom2owl:lifeCycleContribution
  rdf:type owl:ObjectProperty ;
.
lom2owl:lifeCycleContributionRole
  rdf:type owl:DatatypeProperty ;
  rdfs:comment "Kind of contribution. IEEE LOM element 2.3.1."@en ;
  rdfs:domain lom2owl:LifeCycleContribution ;
  rdfs:range [
      rdf:type owl:DataRange ;
      owl:oneOf [
          rdf:type rdf:List ;
          rdf:first "author" ;
          rdf:rest [
              rdf:type rdf:List ;
              rdf:first "content provider" ;
              rdf:rest [
                  rdf:type rdf:List ;
                  rdf:first "editor" ;
                  rdf:rest [
                      rdf:type rdf:List ;
                      rdf:first "educational validator" ;
                      rdf:rest [
                          rdf:type rdf:List ;
                          rdf:first "graphical designer" ;
                          rdf:rest [
                              rdf:type rdf:List ;
                              rdf:first "initiator" ;
                              rdf:rest [
                                  rdf:type rdf:List ;
                                  rdf:first "instructional designer" ;
                                  rdf:rest [
                                      rdf:type rdf:List ;
                                      rdf:first "publisher" ;
                                      rdf:rest [
                                          rdf:type rdf:List ;
                                          rdf:first "script writer" ;
                                          rdf:rest [
                                              rdf:type rdf:List ;
                                              rdf:first "subject matter expert" ;
                                              rdf:rest [
                                                  rdf:type rdf:List ;
                                                  rdf:first "technical implementer" ;
                                                  rdf:rest [
                                                      rdf:type rdf:List ;
                                                      rdf:first "technical validator" ;
                                                      rdf:rest [
                                                          rdf:type rdf:List ;
                                                          rdf:first "terminator" ;
                                                          rdf:rest [
                                                              rdf:type rdf:List ;
                                                              rdf:first "unknown" ;
                                                              rdf:rest [
                                                                  rdf:type rdf:List ;
                                                                  rdf:first "validator" ;
                                                                  rdf:rest () ;
                                                                ] ;
                                                            ] ;
                                                        ] ;
                                                    ] ;
                                                ] ;
                                            ] ;
                                        ] ;
                                    ] ;
                                ] ;
                            ] ;
                        ] ;
                    ] ;
                ] ;
            ] ;
        ] ;
    ] ;
.
lom2owl:lifeCycleStatus
  rdf:type owl:DatatypeProperty ;
  rdfs:comment "The completion status or condition of this learning object. IEEE LOM element 2.2" ;
  rdfs:domain lom2owl:LearningObject ;
  rdfs:range [
      rdf:type owl:DataRange ;
      owl:oneOf [
          rdf:type rdf:List ;
          rdf:first "draft" ;
          rdf:rest [
              rdf:type rdf:List ;
              rdf:first "final" ;
              rdf:rest [
                  rdf:type rdf:List ;
                  rdf:first "revised" ;
                  rdf:rest [
                      rdf:type rdf:List ;
                      rdf:first "unavalaible" ;
                      rdf:rest () ;
                    ] ;
                ] ;
            ] ;
        ] ;
    ] ;
.
lom2owl:lifeCycleVersion
  rdf:type owl:DatatypeProperty ;
  rdfs:domain lom2owl:LearningObject ;
  rdfs:range rdfs:Literal ;
.
lom2owl:metaMetadataContribution
  rdf:type owl:ObjectProperty ;
  rdfs:comment "Those entities (i.e., people, organizations) that have contributed to the state of this learning object during its life cycle (e.g.,creation, edits, publication)."@en ;
  rdfs:domain lom2owl:LearningObject ;
  rdfs:range lom2owl:LifeCycleContribution ;
.
lom2owl:metaMetadataContributionRole
  rdf:type owl:DatatypeProperty ;
  rdfs:comment "Kind of contribution. IEEE LOM element 3.2.1." ;
  rdfs:domain lom2owl:MetaMetadataContribution ;
  rdfs:range xsd:string ;
.
lom2owl:metaMetadataIdentifier
  rdf:type owl:ObjectProperty ;
  rdfs:comment "A globally unique label that identifies this metadata record. IEEE LOM element 3.1." ;
  rdfs:domain lom2owl:LearningObject ;
  rdfs:range lom2owl:Identifier ;
.
lom2owl:metaMetadataLanguage
  rdf:type owl:DatatypeProperty ;
  rdfs:comment "Language of this metadata instance. This is the default language for all LangString values in this metadata instance. If a value for this data element is not present in a metadata instance, then there is no default language for LangString values. IEEE LOM element 3.4."@en ;
  rdfs:domain lom2owl:LearningObject ;
  rdfs:range [
      rdf:type owl:DataRange ;
      owl:oneOf [
          rdf:type rdf:List ;
          rdf:first "ba" ;
          rdf:rest [
              rdf:type rdf:List ;
              rdf:first "ca" ;
              rdf:rest [
                  rdf:type rdf:List ;
                  rdf:first "es" ;
                  rdf:rest [
                      rdf:type rdf:List ;
                      rdf:first "ga" ;
                      rdf:rest () ;
                    ] ;
                ] ;
            ] ;
        ] ;
    ] ;
.
lom2owl:metadataSchema
  rdf:type owl:DatatypeProperty ;
  rdfs:comment "The name and version of the authoritative specification used to create this metadata instance. IEEE LOM element 3.3."@en ;
  rdfs:domain lom2owl:LearningObject ;
  rdfs:range xsd:string ;
.
lom2owl:orCompositeMaximumVersion
  rdf:type owl:DatatypeProperty ;
  rdfs:comment "Highest possible version of the required technology to use the learning object. IEEE LOM element 4.4.1.4."@en ;
  rdfs:domain lom2owl:SingleTechnicalRequirement ;
  rdfs:range xsd:string ;
.
lom2owl:orCompositeMinimumVersion
  rdf:type owl:DatatypeProperty ;
  rdfs:comment "Lowest possible version of the required technology to use the learning object. IEEE LOM element 4.4.1.3."@en ;
  rdfs:domain lom2owl:SingleTechnicalRequirement ;
  rdfs:range xsd:string ;
.
lom2owl:orCompositeName
  rdf:type owl:DatatypeProperty ;
  rdfs:comment "Name of the required technology to use a learning object. IEEE LOM element 4.4.1.2."@en ;
  rdfs:domain lom2owl:SingleTechnicalRequirement ;
  rdfs:range xsd:string ;
.
lom2owl:orCompositeType
  rdf:type owl:DatatypeProperty ;
  rdfs:comment "The technology required to use this learning object, e.g., hardware, software, network, etc. IEEE LOM element 4.4.1.1."@en ;
  rdfs:domain lom2owl:SingleTechnicalRequirement ;
  rdfs:range [
      rdf:type owl:DataRange ;
      owl:oneOf [
          rdf:type rdf:List ;
          rdf:first "browser" ;
          rdf:rest [
              rdf:type rdf:List ;
              rdf:first "operating system" ;
              rdf:rest () ;
            ] ;
        ] ;
    ] ;
.
lom2owl:otherPlatformRequirements
  rdf:type owl:DatatypeProperty ;
  rdfs:domain lom2owl:LearningObject ;
  rdfs:range rdfs:Literal ;
.
lom2owl:relatedResourceDescription
  rdf:type owl:ObjectProperty ;
  terms:description ""^^rdfs:Literal ;
  rdfs:domain lom2owl:Relation ;
  rdfs:range lom2owl:LangString ;
.
lom2owl:relation
  rdf:type owl:ObjectProperty ;
  rdfs:comment "Relationship between a learning object and other learning objects, if any."@en ;
  rdfs:range lom2owl:Relation ;
.
lom2owl:relationKind
  rdf:type owl:DatatypeProperty ;
  rdfs:comment "Nature of the relationship between a learning object and the target learning object, identified by 7.2:Relation.Resource. IEEE LOM element 7.1."@en ;
  rdfs:domain lom2owl:Relation ;
  rdfs:range [
      rdf:type owl:DataRange ;
      owl:oneOf [
          rdf:type rdf:List ;
          rdf:first "hasFormat" ;
          rdf:rest [
              rdf:type rdf:List ;
              rdf:first "hasPart" ;
              rdf:rest [
                  rdf:type rdf:List ;
                  rdf:first "hasVersion" ;
                  rdf:rest [
                      rdf:type rdf:List ;
                      rdf:first "isBasedOn" ;
                      rdf:rest [
                          rdf:type rdf:List ;
                          rdf:first "isBasisFor" ;
                          rdf:rest [
                              rdf:type rdf:List ;
                              rdf:first "isFormatOf" ;
                              rdf:rest [
                                  rdf:type rdf:List ;
                                  rdf:first "isPartOf" ;
                                  rdf:rest [
                                      rdf:type rdf:List ;
                                      rdf:first "isReferencedBy" ;
                                      rdf:rest [
                                          rdf:type rdf:List ;
                                          rdf:first "isRequiredBy" ;
                                          rdf:rest [
                                              rdf:type rdf:List ;
                                              rdf:first "isVersionOf" ;
                                              rdf:rest [
                                                  rdf:type rdf:List ;
                                                  rdf:first "references" ;
                                                  rdf:rest [
                                                      rdf:type rdf:List ;
                                                      rdf:first "requires" ;
                                                      rdf:rest () ;
                                                    ] ;
                                                ] ;
                                            ] ;
                                        ] ;
                                    ] ;
                                ] ;
                            ] ;
                        ] ;
                    ] ;
                ] ;
            ] ;
        ] ;
    ] ;
.
lom2owl:structure
  rdf:type owl:DatatypeProperty ;
  rdfs:comment "Underlying organizational structure of this learning object. IEEE LOM element 1.7."@en ;
  rdfs:domain lom2owl:LearningObject ;
  rdfs:range [
      rdf:type owl:DataRange ;
      owl:oneOf [
          rdf:type rdf:List ;
          rdf:first "atomic" ;
          rdf:rest [
              rdf:type rdf:List ;
              rdf:first "collection" ;
              rdf:rest [
                  rdf:type rdf:List ;
                  rdf:first "hierarchical" ;
                  rdf:rest [
                      rdf:type rdf:List ;
                      rdf:first "linear" ;
                      rdf:rest [
                          rdf:type rdf:List ;
                          rdf:first "networked" ;
                          rdf:rest () ;
                        ] ;
                    ] ;
                ] ;
            ] ;
        ] ;
    ] ;
.
lom2owl:taxonEntry
  rdf:type owl:DatatypeProperty ;
  rdfs:range rdfs:Literal ;
.
lom2owl:taxonId
  rdf:type owl:DatatypeProperty ;
  rdfs:comment "The identifier of the taxon, such as a number or letter combination provided by the source of the taxonomy. IEEE LOM element 9.2.2.1."@en ;
  rdfs:domain lom2owl:Taxon ;
  rdfs:range xsd:string ;
.
lom2owl:taxonPath
  rdf:type owl:ObjectProperty ;
  rdfs:comment "A taxonomic path in a specific classification system according to which a learning object is classified. IEEE LOM element 9.2."@en ;
  rdfs:domain lom2owl:Classification ;
  rdfs:range lom2owl:TaxonPath ;
.
lom2owl:taxonpathSource
  rdf:type owl:DatatypeProperty ;
  rdfs:domain lom2owl:TaxonPath ;
  rdfs:range rdfs:Literal ;
.
lom2owl:technicalDuration
  rdf:type owl:ObjectProperty ;
  rdfs:domain lom2owl:Duration ;
  rdfs:range lom2owl:LearningObject ;
.
lom2owl:technicalInstallationRemarks
  rdf:type owl:DatatypeProperty ;
  rdfs:domain lom2owl:LearningObject ;
  rdfs:range rdfs:Literal ;
.
lom2owl:technicalLocation
  rdf:type owl:DatatypeProperty ;
  rdfs:comment "A string that is used to access this learning object. It may be a location  (e.g., Universal Resource Locator), or a method that resolves to a location (e.g., Universal Resource Identifier). The first element of this list shall be the preferable location. IEEE LOM element 4.3."@en ;
  rdfs:domain lom2owl:LearningObject ;
  rdfs:range xsd:string ;
.
lom2owl:technicalRequirements
  rdf:type owl:ObjectProperty ;
  rdfs:comment "A technical capability necessary for using a learning object. IEEE LOM Element \"4.4. Requirement\"."@en ;
  rdfs:range lom2owl:TechnicalRequirement ;
.
lom2owl:technicalSize
  rdf:type owl:DatatypeProperty ;
  rdfs:comment "The size of the digital learning object in bytes (not Mbytes, GB, etc.). The size is represented as a decimal value. This data element shall refer to the actual size of this learning object. If the learning object is compressed, then this data element shall refer to the uncompressed size. IEEE LOM element 4.2."@en ;
  rdfs:domain lom2owl:LearningObject ;
  rdfs:range xsd:string ;
.
dc:publisher
  rdf:type owl:AnnotationProperty ;
.
terms:coverage
  rdf:type owl:AnnotationProperty ;
.
terms:description
  rdf:type owl:AnnotationProperty ;
.
terms:format
  rdf:type owl:AnnotationProperty ;
.
terms:identifier
  rdf:type owl:AnnotationProperty ;
.
terms:language
  rdf:type owl:AnnotationProperty ;
.
terms:publisher
  rdf:type owl:AnnotationProperty ;
.
terms:rights
  rdf:type owl:AnnotationProperty ;
.
terms:title
  rdf:type owl:AnnotationProperty ;
.
terms:type
  rdf:type owl:AnnotationProperty ;
.
rdf:value
  rdf:type owl:AnnotationProperty ;
.
owl:Thing
  rdf:type owl:Class ;
.
ns:FN
  rdf:type owl:AnnotationProperty ;
.
ns:N
  rdf:type owl:AnnotationProperty ;
.
ns:ORG
  rdf:type owl:AnnotationProperty ;
.
ns:email
  rdf:type owl:AnnotationProperty ;
.
